coq/ZF/Meta/Decl/Axiom/Extensionality.v
@@ -1,0 +1,31 @@
+Require Import Coq.Lists.List.
+Require Import Coq.Strings.String.
+
+Require Import ZF.Meta.Env.
+Require Import ZF.Meta.Syntax.
+Require Import ZF.Meta.Term.Decl.
+Require Import ZF.Meta.Ty.
+
+Import ListNotations.
+
+(* forall a b, (forall x, x :< a <-> x :< b) -> a = b                           *)
+Definition Extensionality : DeclT :=
+  {| paraT := []
+  ;  resT  := TyProp
+  ;  bodyT :=
+      All VarTySet
+        (All VarTySet
+          (Imp
+            (All VarTySet
+              (Iff (Elem (Var 0) (Var 2))
+                   (Elem (Var 0) (Var 1))))
+            (Equal (Var 1) (Var 0))))
+  |}.
+
+Definition imports : Env := Env.empty.
+
+Definition exports : Env := Env.fromListT
+  [ ("Extensionality"%string, Extensionality)
+  ].
+
+Definition env : Env := Env.union imports exports.
